Updated examples to be compatible with label changes

src/single_auth_message/DY.Example.SingleAuthMessage.Protocol.Stateful.Proof.fst
@@ -37,7 +37,7 @@ let state_predicate_protocol: local_state_predicate single_message_state = {
 let all_sessions = [
   pki_tag_and_invariant;
   private_keys_tag_and_invariant;
-  (local_state_single_message_state.tag, local_state_predicate_to_local_bytes_state_predicate state_predicate_protocol);
+  (|local_state_single_message_state.tag, local_state_predicate_to_local_bytes_state_predicate state_predicate_protocol|);
 ]
 
 (**** Event Predicates ****)
@@ -70,8 +70,8 @@ let all_events = [
 
 (**** Create the global trace invariants ****)
 
-let trace_invariants_protocol: trace_invariants (crypto_invariants_protocol) = {
-  state_pred = mk_state_pred crypto_invariants_protocol all_sessions;
+let trace_invariants_protocol: trace_invariants = {
+  state_pred = mk_state_pred all_sessions;
   event_pred = mk_event_pred all_events;
 }
 
@@ -82,35 +82,35 @@ instance protocol_invariants_protocol: protocol_invariants = {
 
 /// Lemmas that the global state predicate contains all the local ones
 
-val all_sessions_has_all_sessions: unit -> Lemma (norm [delta_only [`%all_sessions; `%for_allP]; iota; zeta] (for_allP (has_local_bytes_state_predicate protocol_invariants_protocol) all_sessions))
+val all_sessions_has_all_sessions: unit -> Lemma (norm [delta_only [`%all_sessions; `%for_allP]; iota; zeta] (for_allP has_local_bytes_state_predicate all_sessions))
 let all_sessions_has_all_sessions () =
-  assert_norm(List.Tot.no_repeats_p (List.Tot.map fst (all_sessions)));
-  mk_state_pred_correct protocol_invariants_protocol all_sessions;
-  norm_spec [delta_only [`%all_sessions; `%for_allP]; iota; zeta] (for_allP (has_local_bytes_state_predicate protocol_invariants_protocol) all_sessions)
+  assert_norm(List.Tot.no_repeats_p (List.Tot.map dfst (all_sessions)));
+  mk_state_pred_correct all_sessions;
+  norm_spec [delta_only [`%all_sessions; `%for_allP]; iota; zeta] (for_allP has_local_bytes_state_predicate all_sessions)
 
-val protocol_invariants_protocol_has_pki_invariant: squash (has_pki_invariant protocol_invariants_protocol)
+val protocol_invariants_protocol_has_pki_invariant: squash has_pki_invariant
 let protocol_invariants_protocol_has_pki_invariant = all_sessions_has_all_sessions ()
 
-val protocol_invariants_protocol_has_private_keys_invariant: squash (has_private_keys_invariant protocol_invariants_protocol)
+val protocol_invariants_protocol_has_private_keys_invariant: squash has_private_keys_invariant
 let protocol_invariants_protocol_has_private_keys_invariant = all_sessions_has_all_sessions ()
 
-val protocol_invariants_protocol_has_nsl_session_invariant: squash (has_local_state_predicate protocol_invariants_protocol state_predicate_protocol)
+val protocol_invariants_protocol_has_nsl_session_invariant: squash (has_local_state_predicate state_predicate_protocol)
 let protocol_invariants_protocol_has_nsl_session_invariant = all_sessions_has_all_sessions ()
 
 /// Lemmas that the global event predicate contains all the local ones
 
-val all_events_has_all_events: unit -> Lemma (norm [delta_only [`%all_events; `%for_allP]; iota; zeta] (for_allP (has_compiled_event_pred protocol_invariants_protocol) all_events))
+val all_events_has_all_events: unit -> Lemma (norm [delta_only [`%all_events; `%for_allP]; iota; zeta] (for_allP has_compiled_event_pred all_events))
 let all_events_has_all_events () =
   assert_norm(List.Tot.no_repeats_p (List.Tot.map fst (all_events)));
-  mk_event_pred_correct protocol_invariants_protocol all_events;
-  norm_spec [delta_only [`%all_events; `%for_allP]; iota; zeta] (for_allP (has_compiled_event_pred protocol_invariants_protocol) all_events);
+  mk_event_pred_correct all_events;
+  norm_spec [delta_only [`%all_events; `%for_allP]; iota; zeta] (for_allP has_compiled_event_pred all_events);
   let dumb_lemma (x:prop) (y:prop): Lemma (requires x /\ x == y) (ensures y) = () in
-  dumb_lemma (for_allP (has_compiled_event_pred protocol_invariants_protocol) all_events) (norm [delta_only [`%all_events; `%for_allP]; iota; zeta] (for_allP (has_compiled_event_pred protocol_invariants_protocol) all_events))
+  dumb_lemma (for_allP has_compiled_event_pred all_events) (norm [delta_only [`%all_events; `%for_allP]; iota; zeta] (for_allP has_compiled_event_pred all_events))
 
-val protocol_invariants_has_communication_layer_event_invariants: squash (has_event_pred protocol_invariants_protocol (event_predicate_communication_layer comm_layer_event_preds))
+val protocol_invariants_has_communication_layer_event_invariants: squash (has_event_pred (event_predicate_communication_layer comm_layer_event_preds))
 let protocol_invariants_has_communication_layer_event_invariants = all_events_has_all_events ()
 
-val protocol_invariants_protocol_has_protocol_event_invariant: squash (has_event_pred protocol_invariants_protocol event_predicate_protocol)
+val protocol_invariants_protocol_has_protocol_event_invariant: squash (has_event_pred event_predicate_protocol)
 let protocol_invariants_protocol_has_protocol_event_invariant = all_events_has_all_events ()
 
 (*** Proofs ***)
