src/single_conf_message/DY.Example.SingleConfMessage.Protocol.Stateful.Proof.fst
@@ -16,7 +16,7 @@ let state_predicate_protocol: local_state_predicate single_message_state = {
     match st with
     | SenderState receiver secret -> (
       let sender = prin in
-      get_label secret == join (principal_label sender) (principal_label receiver) /\
+      get_label tr secret == join (principal_label sender) (principal_label receiver) /\
       is_knowable_by (join (principal_label sender) (principal_label receiver)) tr secret
     )
     | ReceiverState secret payload -> (
@@ -43,7 +43,7 @@ let event_predicate_protocol: event_predicate single_message_event =
 let all_sessions = [
   pki_tag_and_invariant;
   private_keys_tag_and_invariant;
-  (local_state_single_message_state.tag, local_state_predicate_to_local_bytes_state_predicate state_predicate_protocol);
+  (|local_state_single_message_state.tag, local_state_predicate_to_local_bytes_state_predicate state_predicate_protocol|);
 ]
 
 /// List of all local event predicates.
@@ -55,9 +55,10 @@ val comm_layer_event_preds: comm_higher_layer_event_preds
 let comm_layer_event_preds = {
   default_comm_higher_layer_event_preds with
   send_conf = (fun sender receiver payload tr -> 
-    exists secret.
+    match decode_message payload with
+    | None -> False
+    | Some {secret} -> (
       event_triggered tr sender (SenderSendMsg sender receiver secret) /\
-      decode_message payload == Some {secret} /\
 
       // The user of the communication layer can
       // also use this function to demand specific
@@ -70,6 +71,7 @@ let comm_layer_event_preds = {
       // (principal_label receiver)) tr secret \/
       // is_publishable tr payload);` 
       is_secret (join (principal_label sender) (principal_label receiver)) tr secret
+    )
   )
 }
 
@@ -80,8 +82,8 @@ let all_events = [
 
 /// Create the global trace invariants.
 
-let trace_invariants_protocol: trace_invariants (crypto_invariants_protocol) = {
-  state_pred = mk_state_pred crypto_invariants_protocol all_sessions;
+let trace_invariants_protocol: trace_invariants = {
+  state_pred = mk_state_pred all_sessions;
   event_pred = mk_event_pred all_events;
 }
 
@@ -92,35 +94,35 @@ instance protocol_invariants_protocol: protocol_invariants = {
 
 /// Lemmas that the global state predicate contains all the local ones
 
-val all_sessions_has_all_sessions: unit -> Lemma (norm [delta_only [`%all_sessions; `%for_allP]; iota; zeta] (for_allP (has_local_bytes_state_predicate protocol_invariants_protocol) all_sessions))
+val all_sessions_has_all_sessions: unit -> Lemma (norm [delta_only [`%all_sessions; `%for_allP]; iota; zeta] (for_allP has_local_bytes_state_predicate all_sessions))
 let all_sessions_has_all_sessions () =
-  assert_norm(List.Tot.no_repeats_p (List.Tot.map fst (all_sessions)));
-  mk_state_pred_correct protocol_invariants_protocol all_sessions;
-  norm_spec [delta_only [`%all_sessions; `%for_allP]; iota; zeta] (for_allP (has_local_bytes_state_predicate protocol_invariants_protocol) all_sessions)
+  assert_norm(List.Tot.no_repeats_p (List.Tot.map dfst (all_sessions)));
+  mk_state_pred_correct all_sessions;
+  norm_spec [delta_only [`%all_sessions; `%for_allP]; iota; zeta] (for_allP has_local_bytes_state_predicate all_sessions)
 
-val protocol_invariants_protocol_has_pki_invariant: squash (has_pki_invariant protocol_invariants_protocol)
+val protocol_invariants_protocol_has_pki_invariant: squash has_pki_invariant
 let protocol_invariants_protocol_has_pki_invariant = all_sessions_has_all_sessions ()
 
-val protocol_invariants_protocol_has_private_keys_invariant: squash (has_private_keys_invariant protocol_invariants_protocol)
+val protocol_invariants_protocol_has_private_keys_invariant: squash has_private_keys_invariant
 let protocol_invariants_protocol_has_private_keys_invariant = all_sessions_has_all_sessions ()
 
-val protocol_invariants_protocol_has_nsl_session_invariant: squash (has_local_state_predicate protocol_invariants_protocol state_predicate_protocol)
+val protocol_invariants_protocol_has_nsl_session_invariant: squash (has_local_state_predicate state_predicate_protocol)
 let protocol_invariants_protocol_has_nsl_session_invariant = all_sessions_has_all_sessions ()
 
 /// Lemmas that the global event predicate contains all the local ones
 
-val all_events_has_all_events: unit -> Lemma (norm [delta_only [`%all_events; `%for_allP]; iota; zeta] (for_allP (has_compiled_event_pred protocol_invariants_protocol) all_events))
+val all_events_has_all_events: unit -> Lemma (norm [delta_only [`%all_events; `%for_allP]; iota; zeta] (for_allP has_compiled_event_pred all_events))
 let all_events_has_all_events () =
   assert_norm(List.Tot.no_repeats_p (List.Tot.map fst (all_events)));
-  mk_event_pred_correct protocol_invariants_protocol all_events;
-  norm_spec [delta_only [`%all_events; `%for_allP]; iota; zeta] (for_allP (has_compiled_event_pred protocol_invariants_protocol) all_events);
+  mk_event_pred_correct all_events;
+  norm_spec [delta_only [`%all_events; `%for_allP]; iota; zeta] (for_allP has_compiled_event_pred all_events);
   let dumb_lemma (x:prop) (y:prop): Lemma (requires x /\ x == y) (ensures y) = () in
-  dumb_lemma (for_allP (has_compiled_event_pred protocol_invariants_protocol) all_events) (norm [delta_only [`%all_events; `%for_allP]; iota; zeta] (for_allP (has_compiled_event_pred protocol_invariants_protocol) all_events))
+  dumb_lemma (for_allP has_compiled_event_pred all_events) (norm [delta_only [`%all_events; `%for_allP]; iota; zeta] (for_allP has_compiled_event_pred all_events))
 
-val protocol_invariants_has_communication_layer_event_invariants: squash (has_event_pred protocol_invariants_protocol (event_predicate_communication_layer comm_layer_event_preds))
+val protocol_invariants_has_communication_layer_event_invariants: squash (has_event_pred (event_predicate_communication_layer comm_layer_event_preds))
 let protocol_invariants_has_communication_layer_event_invariants = all_events_has_all_events ()
 
-val protocol_invariants_protocol_has_nsl_event_invariant: squash (has_event_pred protocol_invariants_protocol event_predicate_protocol)
+val protocol_invariants_protocol_has_nsl_event_invariant: squash (has_event_pred event_predicate_protocol)
 let protocol_invariants_protocol_has_nsl_event_invariant = all_events_has_all_events ()
 
 (*** Proofs ***)
@@ -160,8 +162,8 @@ let send_message_proof tr comm_keys_ids sender receiver state_id =
     let payload = compute_message secret in
     
     let ((), tr) = trigger_event sender (SenderSendMsg sender receiver secret) tr in
-    assert(has_communication_layer_invariants crypto_invariants_protocol);
-    assert(has_communication_layer_event_predicates protocol_invariants_protocol comm_layer_event_preds);
+    assert(has_communication_layer_invariants);
+    assert(has_communication_layer_event_predicates comm_layer_event_preds);
     assert(is_secret (join (principal_label sender) (principal_label receiver)) tr secret);
     send_confidential_proof tr comm_layer_event_preds comm_keys_ids sender receiver payload;
     let (Some msg_id, tr) = send_confidential comm_keys_ids sender receiver payload tr in
@@ -196,8 +198,9 @@ let receive_message_proof tr comm_keys_ids receiver msg_id =
     // `comm_layer_event_preds.send_conf`
     // predicate guarantees this label of `secret`
     // on the sender side.
+    FStar.Classical.move_requires (parse_wf_lemma single_message (is_publishable tr)) payload;
     assert(exists sender. is_secret (join (principal_label sender) (principal_label receiver)) tr secret \/
-      is_publishable tr payload);
+      is_publishable tr secret);
     let (state_id, tr) = new_session_id receiver tr in
     let ((), tr) = set_state receiver state_id (ReceiverState secret payload) tr in
     assert(tr_out == tr);
