src/single_conf_message/DY.Example.SingleConfMessage.Protocol.Total.Proof.fst
@@ -13,20 +13,20 @@ open DY.Example.SingleConfMessage.Protocol.Stateful
 val crypto_usages_protocol: crypto_usages
 instance crypto_usages_protocol = default_crypto_usages
 
-val pkenc_pred_list_protocol: list (string & pkenc_crypto_predicate crypto_usages_protocol)
+val pkenc_pred_list_protocol: list (string & pkenc_crypto_predicate)
 let pkenc_pred_list_protocol = [
   pkenc_crypto_predicates_communication_layer_and_tag
 ]
 
-val sign_pred_list_protocol: list (string & sign_crypto_predicate crypto_usages_protocol)
+val sign_pred_list_protocol: list (string & sign_crypto_predicate)
 let sign_pred_list_protocol = [
   sign_crypto_predicates_communication_layer_and_tag;
 ]
 
 #push-options "--ifuel 2 --fuel 0"
-val crypto_predicates_protocol: crypto_predicates crypto_usages_protocol
+val crypto_predicates_protocol: crypto_predicates
 let crypto_predicates_protocol = {
-  default_crypto_predicates crypto_usages_protocol with
+  default_crypto_predicates with
 
   pkenc_pred = mk_pkenc_predicate pkenc_pred_list_protocol;
 
@@ -45,13 +45,13 @@ val pkenc_pred_has_all_pkenc_preds:
   Lemma
   (ensures
     norm [delta_only [`%pkenc_pred_list_protocol; `%for_allP]; iota; zeta] (
-      for_allP (has_pkenc_predicate crypto_invariants_protocol) pkenc_pred_list_protocol
+      for_allP has_pkenc_predicate pkenc_pred_list_protocol
     )
   )
 let pkenc_pred_has_all_pkenc_preds () =
   assert_norm(List.Tot.no_repeats_p (List.Tot.map fst (pkenc_pred_list_protocol)));
-  mk_pkenc_predicate_correct crypto_invariants_protocol pkenc_pred_list_protocol;
-  norm_spec [delta_only [`%pkenc_pred_list_protocol; `%for_allP]; iota; zeta] (for_allP (has_pkenc_predicate crypto_invariants_protocol) pkenc_pred_list_protocol);
+  mk_pkenc_predicate_correct pkenc_pred_list_protocol;
+  norm_spec [delta_only [`%pkenc_pred_list_protocol; `%for_allP]; iota; zeta] (for_allP has_pkenc_predicate pkenc_pred_list_protocol);
   ()
 
 val sign_pred_has_all_sign_preds:
@@ -59,17 +59,17 @@ val sign_pred_has_all_sign_preds:
   Lemma
   (ensures
     norm [delta_only [`%sign_pred_list_protocol; `%for_allP]; iota; zeta] (
-      for_allP (has_sign_predicate crypto_invariants_protocol) sign_pred_list_protocol
+      for_allP has_sign_predicate sign_pred_list_protocol
     )
   )
 let sign_pred_has_all_sign_preds () =
   assert_norm(List.Tot.no_repeats_p (List.Tot.map fst (sign_pred_list_protocol)));
-  mk_sign_predicate_correct crypto_invariants_protocol sign_pred_list_protocol;
-  norm_spec [delta_only [`%sign_pred_list_protocol; `%for_allP]; iota; zeta] (for_allP (has_sign_predicate crypto_invariants_protocol) sign_pred_list_protocol);
+  mk_sign_predicate_correct sign_pred_list_protocol;
+  norm_spec [delta_only [`%sign_pred_list_protocol; `%for_allP]; iota; zeta] (for_allP has_sign_predicate sign_pred_list_protocol);
   ()
 #pop-options
 
-val protocol_crypto_invariants_has_communication_layer_invariants: squash (has_communication_layer_invariants crypto_invariants_protocol)
+val protocol_crypto_invariants_has_communication_layer_invariants: squash has_communication_layer_invariants
 let protocol_crypto_invariants_has_communication_layer_invariants =
   pkenc_pred_has_all_pkenc_preds ();
   sign_pred_has_all_sign_preds ();
@@ -99,8 +99,7 @@ val decode_message_proof:
   msg_bytes:bytes ->
   Lemma
   (requires
-    is_knowable_by (principal_label receiver) tr msg_bytes \/
-    is_publishable tr msg_bytes
+    is_knowable_by (principal_label receiver) tr msg_bytes
   )
   (ensures (
     match decode_message msg_bytes with
